Fix and tweak checks when sealing and unsealing
Add some missing in-bounds checks.

For sentries, the execute permission strictly speaking doesn't need to
be checked upon creation, but upon invocation.

Also tweak some proof rules to handle common patterns in (un)sealing
instructions.

model/Capabilities_lemmas.thy
@@ -15,7 +15,8 @@ inductive_set derivable :: "'cap set \<Rightarrow> 'cap set" for C :: "'cap set"
 | Unseal:
     "\<lbrakk>c' \<in> derivable C; c'' \<in> derivable C; is_tagged_method CC c'; is_tagged_method CC c'';
       \<not>is_sealed_method CC c''; is_sealed_method CC c'; permits_unseal_method CC c'';
-      get_obj_type_method CC c' = get_cursor_method CC c''\<rbrakk> \<Longrightarrow>
+      get_obj_type_method CC c' = get_cursor_method CC c'';
+      get_cursor_method CC c'' \<in> get_mem_region CC c''\<rbrakk> \<Longrightarrow>
      clear_global_unless CC (is_global_method CC c'') (unseal_method CC c') \<in> derivable C"
 | Seal:
     "\<lbrakk>c' \<in> derivable C; c'' \<in> derivable C; is_tagged_method CC c'; is_tagged_method CC c'';
@@ -23,8 +24,8 @@ inductive_set derivable :: "'cap set \<Rightarrow> 'cap set" for C :: "'cap set"
       permits_seal_method CC c''; get_cursor_method CC c'' \<in> get_mem_region CC c''\<rbrakk> \<Longrightarrow>
      seal_method CC c' (get_cursor_method CC c'') \<in> derivable C"
 | SealEntry:
-    "\<lbrakk>c' \<in> derivable C; \<not>is_sealed_method CC c'; permits_execute_method CC c';
-      is_sentry_method CC (seal_method CC c' otype)\<rbrakk> \<Longrightarrow>
+    "\<lbrakk>c' \<in> derivable C; is_tagged_method CC c';
+      \<not>is_sealed_method CC c'; is_sentry_method CC (seal_method CC c' otype)\<rbrakk> \<Longrightarrow>
      seal_method CC c' otype \<in> derivable C"
 
 lemma leq_cap_refl[simp, intro]:
